fix rep hook override

theories/lithium/solvers.v
@@ -224,3 +224,278 @@ Tactic Notation "solve_goal" :=
   solve_goal with solve_goal_final_hook.
 
 
+(** rep
+
+ The [rep] tactic is an alternative to the [repeat] and [do] tactics
+ that supports left-biased depth-first branching with optional
+ backtracking on failure. *)
+
+(* A backtrack point marker *)
+Definition BACKTRACK_POINT {A} (P : A) : A := P.
+Arguments BACKTRACK_POINT : simpl never.
+Global Typeclasses Opaque BACKTRACK_POINT.
+
+(* For instance, we could redefine the hook as follows: *)
+(*
+Ltac rep_check_backtrack_point_hook ::=
+  match goal with
+    | |- BACKTRACK_POINT ?P =>
+      idtac
+  end.
+ *)
+
+Module Rep.
+  Import Ltac2.
+  Import Ltac2.Printf.
+
+  (* Check whether the current goal is a backtracking point *)
+  Ltac2 rep_check_backtrack_point (x : unit) : bool :=
+    let tac_res := Control.focus 1 1 (fun _ => Control.case (fun _ => ltac1:(rep_check_backtrack_point_hook))) in
+    match tac_res with
+    | Err _ => false
+    | Val _ => true
+    end.
+
+  (* Backtracking mode:
+     - NoBacktrack: don't backtrack
+     - BacktrackSteps n: backtrack to n steps before failure
+     - BacktrackPoint n: go back to the n-th last goal for which [rep_check_backtrack_point] succeeded *)
+  Ltac2 Type backtrack_mode := [ NoBacktrack | BacktrackSteps (int) | BacktrackPoint (int) ].
+
+  (* Exception to signal how many more steps should be backtracked*)
+  Ltac2 Type exn ::= [ RepBacktrack (backtrack_mode) ].
+
+  (* calls [tac] [n] times (n = None means infinite) on the first goal
+  under focus, stops on failure of [tac] and then backtracks according to [nback]. *)
+  Ltac2 rec rep (n : int option) (nback : backtrack_mode) (tac : (unit -> unit)) : int :=
+    (* if there are no goals left, we are done *)
+    match Control.case (fun _ => Control.focus 1 1 (fun _ => ())) with
+    | Err _ => 0
+    | Val _ =>
+      (* check if we should do another repetition *)
+      let do_rep := match n with | None => true | Some n => Int.gt n 0 end in
+      match do_rep with
+      | false => 0
+      | true =>
+        (* maybe we should match on the goal here *)
+        let is_backtrack_point := Control.focus 1 1 (fun _ => rep_check_backtrack_point ()) in
+        (* backtracking point *)
+        let res := Control.case (fun _ =>
+          (* run tac on the first goal *)
+          let tac_res := Control.focus 1 1 (fun _ => Control.case tac) in
+          match tac_res  with
+          | Err _ =>
+              (* if tac failed, start the backtracking *)
+              Control.zero (RepBacktrack nback)
+          | Val _ =>
+              (* compute new n and recurse *)
+              let new_n :=
+                match n with | None => None | Some n => Some (Int.sub n 1) end in
+              let n_steps := rep new_n nback tac in
+              Int.add n_steps 1
+          end) in
+        match res with
+        | Err e =>
+            match e with
+            (* check if we have to backtrack *)
+            | RepBacktrack m =>
+                match m with
+                | BacktrackSteps n =>
+                  (* either rethrow it with one less or return 0 *)
+                  match Int.gt n 0 with
+                  | true => Control.zero (RepBacktrack (BacktrackSteps (Int.sub n 1)))
+                  | false => 0
+                  end
+                | BacktrackPoint n =>
+                    match Int.gt n 0 with
+                    | true =>
+                      (* check if we are at the last backtracking point or rethrow it *)
+                      match is_backtrack_point with
+                      | true =>
+                        match Int.gt n 1 with
+                        | true =>
+                          Control.zero (RepBacktrack (BacktrackPoint (Int.sub n 1)))
+                        | false => 0
+                        end
+                      | false => Control.zero (RepBacktrack (BacktrackPoint n))
+                      end
+                    | false => 0
+                    end
+                | NoBacktrack => 0
+                end
+            | _ => Control.zero e
+            end
+        | Val (r, _) => r
+        end
+      end
+    end.
+
+  Ltac2 print_steps (n : int) :=
+    printf "Did %i steps." n.
+
+  Ltac2 rec pos_to_ltac2_int (n : constr) : int :=
+    lazy_match! n with
+    | xH => 1
+    | xO ?n => Int.mul (pos_to_ltac2_int n) 2
+    | xI ?n => Int.add (Int.mul (pos_to_ltac2_int n) 2) 1
+    end.
+
+  Ltac2 rec z_to_ltac2_int (n : constr) : int :=
+    lazy_match! n with
+    | Z0 => 0
+    | Z.pos ?n => pos_to_ltac2_int n
+    | Z.neg ?n => Int.neg (pos_to_ltac2_int n)
+    end.
+
+  (* TODO: use a mutable record field, see Janno's message *)
+
+  (* Calls tac on a new subgoal of type Z and converts the resulting Z
+  to an int. *)
+  Ltac2 int_from_z_subgoal (tac : unit -> unit) : int :=
+    let x := Control.focus 1 1 (fun _ =>
+      let x := open_constr:(_ : Z) in
+      match Constr.Unsafe.kind x with
+      | Constr.Unsafe.Cast x _ _ =>
+          match Constr.Unsafe.kind x with
+          | Constr.Unsafe.Evar e _ =>
+              Control.new_goal e;
+              x
+          | _ => Control.throw Assertion_failure
+          end
+      | _ => Control.throw Assertion_failure
+      end) in
+    (* new goal has index 2 because it was added after goal number 1 *)
+    Control.focus 2 2 (fun _ =>
+      tac ();
+      (* check that the goal is closed *)
+      Control.enter (fun _ => Control.throw Assertion_failure));
+    Control.focus 1 1 (fun _ =>
+      let x := Std.eval_vm None x in
+      z_to_ltac2_int x).
+
+  (* Necessary because Some and None cannot be used in ltac2: quotations. *)
+  Ltac2 some (n : int) : int option := Some n.
+  Ltac2 none : int option := None.
+End Rep.
+
+(** rep repeatedly applies tac to the goal in a depth-first manner. In
+particular, if tac generates multiple subgoals, the process continues
+with the first subgoal and only looks at the second subgoal if the
+first subgoal (and all goals spawed from it) are solved. If [tac]
+fails, the complete process stops (unlike [repeat] which continues
+with other subgoals).
+
+[rep n tac] iterates this process at most n times.
+[rep <- n tac] backtracks n steps on failure.
+[rep <-! tac] backtracks to the last backtracking point on failure.
+ (See the comment on [rep_check_backtrack_point] above to see what a backtracking point is)
+[rep <-? n tac] backtracks to the n-th last backtracking point on failure.
+*)
+Tactic Notation "rep" tactic3(tac) :=
+  let r := ltac2:(tac |-
+    Rep.print_steps (Rep.rep Rep.none Rep.NoBacktrack (fun _ => Ltac1.run tac))) in
+  r tac.
+
+(* rep is carefully written such that all goals are passed to Ltac2
+and rep can apply tac in a depth-first manner to only the first goal.
+In particular, the behavior of [all: rep 10 tac.] is equivalent to
+[all: rep 5 tac. all: rep 5 tac.], even if the first call spawns new
+subgoals. (See also the tests.) *)
+Tactic Notation "rep" int(n) tactic3(tac) :=
+  let ntac := do n (refine (1 + _)%Z); refine 0%Z in
+  let r := ltac2:(ntac tac |-
+    let n := Rep.int_from_z_subgoal (fun _ => Ltac1.run ntac) in
+    Rep.print_steps (Rep.rep (Rep.some n) Rep.NoBacktrack (fun _ => Ltac1.run tac))) in
+  r ntac tac.
+
+Tactic Notation "rep" "<-" int(n) tactic3(tac) :=
+  let ntac := do n (refine (1 + _)%Z); refine 0%Z in
+  let r := ltac2:(ntac tac |-
+     let n := Rep.int_from_z_subgoal (fun _ => Ltac1.run ntac) in
+     Rep.print_steps (Rep.rep (Rep.none) (Rep.BacktrackSteps n) (fun _ => Ltac1.run tac))) in
+  r ntac tac.
+
+Tactic Notation "rep" "<-!" tactic3(tac) :=
+  let r := ltac2:(tac |-
+    Rep.print_steps (Rep.rep Rep.none (Rep.BacktrackPoint 1) (fun _ => Ltac1.run tac))) in
+  r tac.
+
+Tactic Notation "rep" "<-?" int(n) tactic3(tac) :=
+  let ntac := do n (refine (1 + _)%Z); refine 0%Z in
+  let r := ltac2:(ntac tac |-
+     let n := Rep.int_from_z_subgoal (fun _ => Ltac1.run ntac) in
+     Rep.print_steps (Rep.rep (Rep.none) (Rep.BacktrackPoint n) (fun _ => Ltac1.run tac))) in
+  r ntac tac.
+
+Module RepTest.
+  Definition DELAY (P : Prop) : Prop := P.
+
+  Ltac DELAY_test_tac :=
+    first [
+        lazymatch goal with | |- DELAY ?P => change P end |
+        exact eq_refl |
+        split |
+        lazymatch goal with | |- BACKTRACK_POINT ?P => change P end
+      ].
+  Local Ltac rep_check_backtrack_point_hook ::=
+    match goal with
+    | |- BACKTRACK_POINT ?P =>
+      idtac
+    end.
+
+  Goal ∃ x, Nat.iter 10 DELAY (x = 1) ∧ Nat.iter 6 DELAY (x = 2). simpl. eexists.
+    all: rep DELAY_test_tac.
+    1: lazymatch goal with | |- 1 = 2 => idtac | |- _ => fail "unexpected goal" end.
+  Abort.
+
+  Goal ∃ x, Nat.iter 10 DELAY (x = 1) ∧ Nat.iter 6 DELAY (x = 2). simpl. eexists.
+    all: rep 5 DELAY_test_tac.
+    1: lazymatch goal with | |- DELAY (DELAY (DELAY (DELAY (DELAY (DELAY (_ = 1)))))) => idtac | |- _ => fail "unexpected goal" end.
+    2: lazymatch goal with | |- DELAY (DELAY (DELAY (DELAY (DELAY (DELAY (_ = 2)))))) => idtac | |- _ => fail "unexpected goal" end.
+    (* This should only apply tac to the first subgoal. *)
+    all: rep 5 DELAY_test_tac.
+    1: lazymatch goal with | |- DELAY (_ = 1) => idtac | |- _ => fail "unexpected goal" end.
+    2: lazymatch goal with | |- DELAY (DELAY (DELAY (DELAY (DELAY (DELAY (_ = 2)))))) => idtac | |- _ => fail "unexpected goal" end.
+    (* This finishes the first subgoal and use the remaining steps on
+    the second subgoal. *)
+    all: rep 5 DELAY_test_tac.
+    1: lazymatch goal with | |- DELAY (DELAY (DELAY (1 = 2))) => idtac | |- _ => fail "unexpected goal" end.
+  Abort.
+
+  Goal ∃ x, Nat.iter 10 DELAY (x = 1) ∧ Nat.iter 6 DELAY (x = 2). simpl. eexists.
+    repeat DELAY_test_tac.
+    (* Same as rep above. *)
+  Abort.
+
+  Goal ∃ x, Nat.iter 10 DELAY (x = 1) ∧ Nat.iter 6 DELAY (x = 2). simpl. eexists.
+    do 5? (DELAY_test_tac).
+    (* Notice the difference to [rep] above: [do] also applies the
+    steps to the second subgoal. *)
+  Abort.
+
+  Goal ∃ x, Nat.iter 10 DELAY (x ≤ 1) ∧ Nat.iter 6 DELAY (x = 2). simpl. eexists.
+    rep <-3 DELAY_test_tac.
+    1: lazymatch goal with | |- DELAY (DELAY (DELAY (_ ≤ 1))) => idtac | |- _ => fail "unexpected goal" end.
+    2: lazymatch goal with | |- DELAY (DELAY (DELAY (DELAY (DELAY (DELAY (_ = 2)))))) => idtac | |- _ => fail "unexpected goal" end.
+  Abort.
+
+  Goal ∃ x, Nat.iter 10 DELAY (x ≤ 1) ∧ Nat.iter 6 DELAY (x = 2). simpl. eexists.
+    repeat DELAY_test_tac.
+    (* Notice the difference to [rep] above: [repeat] continues with
+    the second subgoal on failure. *)
+  Abort.
+
+  Goal BACKTRACK_POINT (Nat.iter 10 DELAY (BACKTRACK_POINT (BACKTRACK_POINT (Nat.iter 10 DELAY (1 = 2))))). simpl.
+    all: rep <-! DELAY_test_tac.
+    all: do 11 DELAY_test_tac.
+    1: lazymatch goal with | |- 1 = 2 => idtac | |- _ => fail "unexpected goal" end.
+  Abort.
+
+  Goal BACKTRACK_POINT (Nat.iter 10 DELAY (BACKTRACK_POINT (BACKTRACK_POINT (Nat.iter 10 DELAY (1 = 2))))). simpl.
+    all: rep <-? 3 DELAY_test_tac.
+    all: do 23 DELAY_test_tac.
+    1: lazymatch goal with | |- 1 = 2 => idtac | |- _ => fail "unexpected goal" end.
+  Abort.
+
+End RepTest.
+
